BlockLayer refactor into CrashTolerant subcomponents complete

Splinter/BlockLayer/BlockCoordinationSystem.i.dfy
@@ -1,85 +1,64 @@
 // Copyright 2018-2021 VMware, Inc., Microsoft Inc., Carnegie Mellon University, ETH Zurich, and University of Washington
 // SPDX-License-Identifier: BSD-2-Clause
 
-include "../../Spec/MapSpec.s.dfy"
-include "../CoordinationLayer/AbstractMap.i.dfy"
-include "../Journal/MarshalledJournal.i.dfy"
+include "../CoordinationLayer/CoordinationSystem.i.dfy"
+include "BlockCrashTolerantJournal.i.dfy"
+include "BlockCrashTolerantMap.i.dfy"
 
 // TODO(jonh,robj): This file consists largely of copy-pastage from CoordinationSystem.
 // Figure out how to refactor; maybe create subpredicates in CoordinationSystem to reuse here?
-module BlockCoordinationSystem
-{
+// Or maybe now it's just functor re-use.
+// Or maybe it'll get interesting because we're going to begin talking about framing finally.
+
+module BlockCoordinationSystem {
   import opened Options
   import opened MapRemove_s
+  import opened CrashTolerantMapSpecMod
+  import opened StampedMapMod
   import opened MsgHistoryMod
-  import opened LSNMod
   import opened KeyType
   import opened ValueMessage
   import opened TotalKMMapMod
-  import opened CrashTolerantMapSpecMod
-  import opened StampedMapMod
-  import opened MarshalledJournal
-  import opened GenericDisk
-  import opened AbstractMap
+  import opened LSNMod
+  import opened BlockCrashTolerantJournal
+  import opened BlockCrashTolerantMap
+  import CoordinationSystem
 
   import Async = CrashTolerantMapSpecMod.uiopifc.async
   type UIOp = CrashTolerantMapSpecMod.uiopifc.UIOp
+
   type SyncReqs = map<CrashTolerantMapSpecMod.uiopifc.SyncReqId, LSN>
-
-  // This DiskImage corresponds to the datatype by the same name way up at the
-  // CoordinationSystem layer. In the implementation it represents the superblock
-  // and all the blocks reachable from the superblock.
-  datatype DiskImage = DiskImage(
-    mapadt: StampedMap,
-    journal: JournalImage)
-  {
-    predicate WF() {
-      && journal.WF()
-    }
-
-    function SeqEnd() : LSN
-      requires WF()
-    {
-      journal.SeqEnd()
-    }
-
-    predicate CompletesSync(lsn: LSN)
-      requires WF()
-    {
-      lsn < SeqEnd()
-    }
-  }
 
   datatype Ephemeral =
     | Unknown
     | Known(
       progress: Async.EphemeralState,
       syncReqs: SyncReqs,
-
-      mapadt: AbstractMap.Variables,
-      mapLsn: LSN,  // invariant: agrees with mapadt.stampedMap.seqEnd
-      journal: MarshalledJournal.Variables,
-
-      frozenMap: Option<StampedMap>
+      mapLsn: LSN  // invariant: agrees with mapadt.stampedMap.seqEnd
     )
   {
-    predicate WF() {
-      Known? ==> (
-        && true
-      )
-    }
   }
 
   datatype Variables = Variables(
-    persistentImage: DiskImage,
-    ephemeral: Ephemeral,
-    inFlightImage: Option<DiskImage>
+    journal: BlockCrashTolerantJournal.Variables,
+    mapadt: BlockCrashTolerantMap.Variables,
+    ephemeral: Ephemeral
   )
   {
-    predicate WF() {
-      && persistentImage.WF()
-      && (ephemeral.Known? ==> ephemeral.WF())
-      && (inFlightImage.Some? ==> inFlightImage.value.WF())
+    predicate WF()
+    {
+      && journal.WF()
+      && mapadt.WF()
+      && (ephemeral.Known? == journal.ephemeral.Known? == mapadt.ephemeral.Known?)
+      // Provable from invariant:
+      && (journal.inFlight.Some? ==> mapadt.inFlight.Some?)
+    }
+
+    predicate Init()
+    {
+      && BlockCrashTolerantJournal.Init(journal)
+      && BlockCrashTolerantMap.Init(mapadt)
+      && ephemeral.Unknown?
     }
   }
 
@@ -87,22 +66,16 @@ module BlockCoordinationSystem
   {
     && v.WF()
     && uiop.NoopOp?
-    && v.ephemeral.Unknown?
     && v'.ephemeral.Known?
-    && MarshalledJournal.Init(v'.ephemeral.journal, v.persistentImage.journal)
-    && AbstractMap.Init(v'.ephemeral.mapadt, v.persistentImage.mapadt)
-    && v' == v.(ephemeral := Known(
-      Async.InitEphemeralState(),
-      map[],  // syncReqs
-      v'.ephemeral.mapadt, // defined by predicate update update
-      v.persistentImage.mapadt.seqEnd,
-      v'.ephemeral.journal, // defined by predicate update update
-      None  // frozen map
-      ))
+    && BlockCrashTolerantJournal.Next(v.journal, v'.journal, CrashTolerantJournal.LoadEphemeralFromPersistentLabel())
+    && BlockCrashTolerantMap.Next(v.mapadt, v'.mapadt, CrashTolerantMap.LoadEphemeralFromPersistentLabel(v'.ephemeral.mapLsn))
+    && v'.ephemeral.progress == Async.InitEphemeralState()
+    && v'.ephemeral.syncReqs == map[]
+    // and thus all fields of v' are constrained.
   }
 
   // Move some journal state into the map to make it (closer to) fresh
-  predicate Recover(v: Variables, v': Variables, uiop : UIOp, puts:MsgHistory)
+  predicate Recover(v: Variables, v': Variables, uiop : UIOp, records:MsgHistory)
   {
     && uiop.NoopOp?
     && v.WF()
@@ -110,17 +83,14 @@ module BlockCoordinationSystem
     && v'.WF()
     && v'.ephemeral.Known?
 
-    && puts.WF()
+    && records.WF()
 
     // NB that Recover can interleave with mapadt steps (the Betree
     // reorganizing its state, possibly flushing stuff out to disk).
-    && MarshalledJournal.Next(v.ephemeral.journal, v'.ephemeral.journal, MarshalledJournal.ReadForRecoveryLabel(puts))
-    && AbstractMap.Put(v.ephemeral.mapadt, v'.ephemeral.mapadt, AbstractMap.PutLabel(puts))
-    && v' == v.(ephemeral := v.ephemeral.(
-        journal := v'.ephemeral.journal, // predicate update above
-        mapadt := v'.ephemeral.mapadt,   // predicate update above
-        mapLsn := puts.seqEnd
-      ))
+    && BlockCrashTolerantJournal.Next(v.journal, v'.journal, CrashTolerantJournal.ReadForRecoveryLabel(records))
+    && BlockCrashTolerantMap.Next(v.mapadt, v'.mapadt, CrashTolerantMap.PutRecordsLabel(records))
+
+    && v'.ephemeral == v.ephemeral.(mapLsn := records.seqEnd) // all else defined via predicates above
   }
 
   predicate AcceptRequest(v: Variables, v': Variables, uiop : UIOp)
@@ -151,17 +121,16 @@ module BlockCoordinationSystem
     && var key := uiop.baseOp.req.input.key;
     && var value := uiop.baseOp.reply.output.value;
     && assert AnyKey(key);
-    // Map handles the query
-    && AbstractMap.Query(v.ephemeral.mapadt, v'.ephemeral.mapadt, AbstractMap.QueryLabel(v.ephemeral.mapLsn, key, value))
+
     // Journal confirms that the map is up-to-date (but otherwise doesn't do anything).
-    && MarshalledJournal.Next(v.ephemeral.journal, v'.ephemeral.journal, MarshalledJournal.QueryEndLsnLabel(v.ephemeral.mapLsn))
-    && v' == v.(ephemeral := v.ephemeral.(
-        mapadt := v'.ephemeral.mapadt,  // predicate update above
-        journal := v'.ephemeral.journal,  // predicate update above
-        progress := v.ephemeral.progress.(
+    && BlockCrashTolerantJournal.Next(v.journal, v'.journal, CrashTolerantJournal.QueryEndLsnLabel(v.ephemeral.mapLsn))
+    // Map handles the query
+    && BlockCrashTolerantMap.Next(v.mapadt, v'.mapadt, CrashTolerantMap.QueryLabel(v.ephemeral.mapLsn, key, value))
+
+    && v'.ephemeral == v.ephemeral.(progress := v.ephemeral.progress.(
           requests := v.ephemeral.progress.requests - {uiop.baseOp.req},
           replies := v.ephemeral.progress.replies + {uiop.baseOp.reply}
-      )))
+      ))
   }
 
   predicate Put(v: Variables, v': Variables, uiop : UIOp)
@@ -190,18 +159,17 @@ module BlockCoordinationSystem
     && var singleton := MsgHistoryMod.SingletonAt(v.ephemeral.mapLsn, KeyedMessage(key, Define(val)));
 
     && v.WF()
-    && MarshalledJournal.Next(v.ephemeral.journal, v'.ephemeral.journal, MarshalledJournal.PutLabel(singleton))
-    && AbstractMap.Next(v.ephemeral.mapadt, v'.ephemeral.mapadt, AbstractMap.PutLabel(singleton))
-    && v' == v.(ephemeral := v.ephemeral.(
-          journal := v'.ephemeral.journal,  // predicate update above
-          mapadt := v'.ephemeral.mapadt,  // predicate update above
+    && BlockCrashTolerantJournal.Next(v.journal, v'.journal, CrashTolerantJournal.PutLabel(singleton))
+    && BlockCrashTolerantMap.Next(v.mapadt, v'.mapadt, CrashTolerantMap.PutRecordsLabel(singleton))
+
+    && v'.ephemeral == v.ephemeral.(
           mapLsn := v.ephemeral.mapLsn + 1,
-          // Frozen stuff unchanged here.
           progress := v.ephemeral.progress.(
             requests := v.ephemeral.progress.requests - {uiop.baseOp.req},
             replies := v.ephemeral.progress.replies + {uiop.baseOp.reply}
+          // syncReqs UNCHANGED
           )
-      ))
+      )
   }
 
   predicate DeliverReply(v: Variables, v': Variables, uiop : UIOp)
@@ -217,16 +185,15 @@ module BlockCoordinationSystem
   // Journal Internal steps (writing stuff out to disk, for example)
   // and Betree Internal steps (writing stuff to disk, flushing and compacting,
   // which create new blocks in cache and rearrange the indirection table)
-  // all look like no-ops ("stutter" in Lamport's TLA+ terminology) at this layer.
+  // all look like stutters at this layer.
 
   predicate JournalInternal(v: Variables, v': Variables, uiop : UIOp)
   {
     && v.ephemeral.Known?
     && v'.ephemeral.Known?
     && uiop.NoopOp?
-    && MarshalledJournal.Next(v.ephemeral.journal, v'.ephemeral.journal, MarshalledJournal.InternalLabel())
-    && v' == v.(ephemeral := v.ephemeral.(
-          journal := v'.ephemeral.journal))  // predicate update above
+    && BlockCrashTolerantJournal.Next(v.journal, v'.journal, CrashTolerantJournal.InternalLabel())
+    && v' == v.(journal := v'.journal)  // predicate update above
   }
 
   predicate MapInternal(v: Variables, v': Variables, uiop : UIOp)
@@ -234,9 +201,8 @@ module BlockCoordinationSystem
     && v.ephemeral.Known?
     && v'.ephemeral.Known?
     && uiop.NoopOp?
-    && AbstractMap.Next(v.ephemeral.mapadt, v'.ephemeral.mapadt, AbstractMap.InternalLabel())
-    && v' == v.(ephemeral := v.ephemeral.(
-          mapadt := v'.ephemeral.mapadt))  // predicate update above
+    && BlockCrashTolerantMap.Next(v.mapadt, v'.mapadt, CrashTolerantMap.InternalLabel())
+    && v' == v.(mapadt := v'.mapadt)  // predicate update above
   }
 
   predicate ReqSync(v: Variables, v': Variables, uiop : UIOp)
@@ -247,18 +213,19 @@ module BlockCoordinationSystem
     && v'.ephemeral.Known?
     && uiop.ReqSyncOp?
     && uiop.syncReqId !in v.ephemeral.syncReqs
+
+    // TODO(robj): cleanup: delete this predicate; it's probably totally unecessary.
     // Need to record the current LSN, which is generally the current map state. But we
     // also need to confirm that the journal hasn't gone ahead, since sync is relative to
     // writes (which have affected the journal).
-    && MarshalledJournal.Next(v.ephemeral.journal, v'.ephemeral.journal, MarshalledJournal.QueryEndLsnLabel(v.ephemeral.mapLsn))
-    && AbstractMap.Next(v.ephemeral.mapadt, v'.ephemeral.mapadt, AbstractMap.QueryEndLsnLabel(v.ephemeral.mapLsn))
+    && BlockCrashTolerantJournal.Next(v.journal, v'.journal, CrashTolerantJournal.QueryEndLsnLabel(v.ephemeral.mapLsn))
+
+    && v'.mapadt == v.mapadt
 
     // NB that the label for a sync in the table is the LSN AFTER the last write
-    && v' == v.(ephemeral := v.ephemeral.(
-        journal := v'.ephemeral.journal,  // predicate update above
-        mapadt := v'.ephemeral.mapadt,  // predicate update above
+    && v'.ephemeral == v.ephemeral.(
         syncReqs := v.ephemeral.syncReqs[uiop.syncReqId := v.ephemeral.mapLsn]
-      ))
+      )
   }
 
   predicate ReplySync(v: Variables, v': Variables, uiop : UIOp)
@@ -267,114 +234,56 @@ module BlockCoordinationSystem
     && v.ephemeral.Known?
     && uiop.ReplySyncOp?
     && uiop.syncReqId in v.ephemeral.syncReqs
-    && v.persistentImage.CompletesSync(v.ephemeral.syncReqs[uiop.syncReqId]) // sync lsn is persistent
+    && BlockCrashTolerantJournal.Next(v.journal, v'.journal, CrashTolerantJournal.QueryLsnPersistenceLabel(v.ephemeral.syncReqs[uiop.syncReqId]))
     && v' == v.(ephemeral := v.ephemeral.(
         syncReqs := MapRemove1(v.ephemeral.syncReqs, uiop.syncReqId)
       ))
   }
 
-  predicate FreezeMapAdt(v: Variables, v': Variables, uiop : UIOp)
+  // This step models issuing the superblock write
+  predicate CommitStart(v: Variables, v': Variables, uiop : UIOp, newBoundaryLsn: LSN)
   {
     && uiop.NoopOp?
     && v.WF()
     && v.ephemeral.Known?
-    && v'.ephemeral.Known?
-    // Copy the current map into the frozen one, deleting whatever was
-    // frozen.
-    && v'.ephemeral.frozenMap.Some?
-    && AbstractMap.FreezeAs(v.ephemeral.mapadt, v'.ephemeral.mapadt, AbstractMap.FreezeAsLabel(v'.ephemeral.frozenMap.value))
-    // TODO this should cause mischief if a Commit is in progress. Does it?
-    && v' == v.(ephemeral := v.ephemeral.(
-        mapadt := v'.ephemeral.mapadt,  // predicate update above
-        frozenMap := v'.ephemeral.frozenMap  // predicate update above
-      ))
+
+    && BlockCrashTolerantJournal.Next(v.journal, v'.journal, CrashTolerantJournal.CommitStartLabel(newBoundaryLsn, v.ephemeral.mapLsn))
+    && BlockCrashTolerantMap.Next(v.mapadt, v'.mapadt, CrashTolerantMap.CommitStartLabel(newBoundaryLsn))
+
+    && v'.ephemeral == v.ephemeral  // UNCHANGED
   }
 
-  predicate CommitStart(v: Variables, v': Variables, uiop : UIOp, frozenJournal: JournalImage)
-  {
-    && uiop.NoopOp?
-    && v.WF()
-    && v.ephemeral.Known?
-    && v'.ephemeral.Known?
-    && v.inFlightImage.None?
-
-    && v.ephemeral.frozenMap.Some?
-    && frozenJournal.WF()
-    && v.ephemeral.frozenMap.value.seqEnd == frozenJournal.SeqStart()
-    // Frozen map can't go backwards vs persistent map, lest we end up with
-    // a gap to the ephemeral journal start.
-    && v.persistentImage.mapadt.seqEnd <= frozenJournal.SeqStart()
-    // And of course there should be no way for it to have passed the ephemeral map!
-    && frozenJournal.SeqStart() <= v.ephemeral.mapLsn
-    && v.persistentImage.SeqEnd() <= frozenJournal.SeqEnd()
-
-    && MarshalledJournal.Next(v.ephemeral.journal, v'.ephemeral.journal,
-        MarshalledJournal.FreezeForCommitLabel(frozenJournal))
-    && AbstractMap.Next(v.ephemeral.mapadt, v'.ephemeral.mapadt, AbstractMap.QueryEndLsnLabel(v.ephemeral.mapLsn))
-
-    && v'.inFlightImage.Some?
-    && v' == v.(
-        ephemeral := v.ephemeral.(mapadt := v'.ephemeral.mapadt),  // predicate update above
-        inFlightImage := Some(DiskImage(v.ephemeral.frozenMap.value, frozenJournal)))
-  }
-
+  // This step models learning that the outstanding superblock write has completed.
   predicate CommitComplete(v: Variables, v': Variables, uiop : UIOp)
   {
     && v.WF()
     && v'.WF()
-    && v.ephemeral.Known?
-    && v.inFlightImage.Some?
-    && var ifImage := v.inFlightImage.value;
-
     && uiop.SyncOp?
-    && v'.ephemeral.Known?
+    && v.ephemeral.Known? // provable from invariant
 
-    && MarshalledJournal.Next(v.ephemeral.journal, v'.ephemeral.journal,
-        MarshalledJournal.DiscardOldLabel(ifImage.mapadt.seqEnd, v.ephemeral.mapLsn))
-    && AbstractMap.Next(v.ephemeral.mapadt, v'.ephemeral.mapadt, AbstractMap.QueryEndLsnLabel(v.ephemeral.mapLsn))
+    && BlockCrashTolerantJournal.Next(v.journal, v'.journal, CrashTolerantJournal.CommitCompleteLabel(v.ephemeral.mapLsn))
+    && BlockCrashTolerantMap.Next(v.mapadt, v'.mapadt, CrashTolerantMap.CommitCompleteLabel())
 
-    && v' == v.(
-        persistentImage := ifImage,
-        ephemeral := v.ephemeral.(
-          journal := v'.ephemeral.journal, // predicate update above
-          mapadt := v'.ephemeral.mapadt    // predicate update above
-        ),
-        inFlightImage := None)
+    && v'.ephemeral == v.ephemeral  // UNCHANGED
   }
 
   predicate Crash(v: Variables, v': Variables, uiop : UIOp)
   {
+    && v.WF()
+    && v'.WF()
     && uiop.CrashOp?
-    && v' == v.(ephemeral := Unknown, inFlightImage := None)
+
+    && BlockCrashTolerantJournal.Next(v.journal, v'.journal, CrashTolerantJournal.CrashLabel())
+    && BlockCrashTolerantMap.Next(v.mapadt, v'.mapadt, CrashTolerantMap.CrashLabel())
+
+    && v'.ephemeral.Unknown?
   }
 
-  function MkfsDiskImage() : DiskImage
-  {
-    DiskImage(StampedMapMod.Empty(), MarshalledJournal.Mkfs())
+  predicate Init(v: Variables) {
+    v.Init()
   }
 
-  predicate Init(v: Variables)
-  {
-    && v.persistentImage == MkfsDiskImage()
-    && v.ephemeral.Unknown?
-    && v.inFlightImage.None?
-  }
-
-  datatype Step =
-    | LoadEphemeralFromPersistentStep()
-    | RecoverStep(puts:MsgHistory)
-    | AcceptRequestStep()
-    | QueryStep()
-    | PutStep()
-    | DeliverReplyStep()
-    | JournalInternalStep()
-    | MapInternalStep()
-    | ReqSyncStep()
-    | ReplySyncStep()
-    | FreezeMapAdtStep()
-    | CommitStartStep(frozenJournal: JournalImage)
-    | CommitCompleteStep()
-    | CrashStep()
+  type Step = CoordinationSystem.Step // laaaazy
 
   predicate NextStep(v: Variables, v': Variables, uiop : UIOp, step: Step) {
     match step {
@@ -388,8 +297,7 @@ module BlockCoordinationSystem
       case MapInternalStep() => MapInternal(v, v', uiop)
       case ReqSyncStep() => ReqSync(v, v', uiop)
       case ReplySyncStep() => ReplySync(v, v', uiop)
-      case FreezeMapAdtStep() => FreezeMapAdt(v, v', uiop)
-      case CommitStartStep(frozenJournal) => CommitStart(v, v', uiop, frozenJournal)
+      case CommitStartStep(newBoundaryLsn) => CommitStart(v, v', uiop, newBoundaryLsn)
       case CommitCompleteStep() => CommitComplete(v, v', uiop)
       case CrashStep() => Crash(v, v', uiop)
     }
