Splinter/BlockLayer/BlockCrashTolerantJournalRefinement.i.dfy
@@ -1,0 +1,223 @@
+// Copyright 2018-2021 VMware, Inc., Microsoft Inc., Carnegie Mellon University, ETH Zurich, and University of Washington
+// SPDX-License-Identifier: BSD-2-Clause
+
+include "BlockCrashTolerantJournal.i.dfy"
+include "../Journal/MarshalledJournalRefinement.i.dfy"
+include "../CoordinationLayer/CrashTolerantJournal.i.dfy"
+
+module BlockCrashTolerantJournalRefinement {
+  import opened Options
+  import opened ValueMessage
+  import opened KeyType
+  import opened StampedMapMod
+  import opened MsgHistoryMod
+  import opened LSNMod
+  import CrashTolerantJournal 
+  import PagedJournalRefinement 
+  import AbstractJournal
+  import PagedJournal
+  import LinkedJournal
+  import MarshalledJournal
+  import LinkedJournalRefinement 
+  import MarshalledJournalRefinement 
+  import opened BlockCrashTolerantJournal 
+
+  predicate DecodableImage(store: StoreImage)
+  {
+    && store.WF()
+    && store.I().Decodable()
+  }
+
+  function IImage(store: StoreImage) : CrashTolerantJournal.StoreImage
+    requires DecodableImage(store)
+  {
+    store.I().I().I()
+  }
+
+  function IALabel(lbl: TransitionLabel) : CrashTolerantJournal.TransitionLabel
+    requires lbl.WF()
+  {
+    lbl
+  }
+
+  predicate Decodable(v: Variables)
+  {
+    && DecodableImage(v.persistent)
+    && (v.ephemeral.Known? ==> MarshalledJournalRefinement.Inv(v.ephemeral.v))
+    && (v.inFlight.Some? ==> DecodableImage(v.inFlight.value))
+  }
+
+  function IMJ(mv: MarshalledJournal.Variables) : AbstractJournal.Variables
+    requires mv.WF()
+    requires MarshalledJournalRefinement.Inv(mv)
+  {
+    PagedJournalRefinement.I(LinkedJournalRefinement.I(MarshalledJournalRefinement.I(mv)))
+  }
+
+  function I(v: Variables) : CrashTolerantJournal.Variables
+    requires Decodable(v)
+  {
+    CrashTolerantJournal.Variables(
+      IImage(v.persistent),
+      if v.ephemeral.Unknown?  then CrashTolerantJournal.Unknown else CrashTolerantJournal.Known(IMJ(v.ephemeral.v)),
+      if v.inFlight.None? then None else Some(IImage(v.inFlight.value))
+    )
+  }
+
+  predicate Inv(v: Variables)
+  {
+    && Decodable(v)
+    && (v.ephemeral.Known? ==> v.persistent.I().diskView.IsSubDisk(v.ephemeral.v.journalImage.I().diskView))
+    && (v.inFlight.Some? ==>
+        && v.ephemeral.Known?
+        && LinkedJournalRefinement.InFlightSubDiskProperty(
+            MarshalledJournalRefinement.I(v.ephemeral.v), v.inFlight.value.I())
+      )
+  }
+
+  lemma InitRefines(v: Variables)
+    requires Init(v)
+    ensures Inv(v)
+    ensures CrashTolerantJournal.Init(I(v))
+  {
+    assert v.persistent.I().diskView.PointersRespectRank(map[]);  // Decodable requires Acyclic.
+  }
+
+  // Maybe this belongs in MarshalledJournal specifically?
+  predicate DecodableMJLabel(lbl: MarshalledJournal.TransitionLabel) {
+    && lbl.WF()
+    && lbl.I().WF()
+  }
+  function IAMJLabel(lbl: MarshalledJournal.TransitionLabel) : AbstractJournal.TransitionLabel
+    requires DecodableMJLabel(lbl)
+  {
+    PagedJournalRefinement.ILbl(lbl.I().I())
+  }
+
+  lemma LoadEphemeralFromPersistentRefines(v: Variables, v': Variables, lbl: TransitionLabel)
+    requires Inv(v) && Next(v, v', lbl) && lbl.LoadEphemeralFromPersistentLabel?
+    ensures Inv(v') && CrashTolerantJournal.Next(I(v), I(v'), IALabel(lbl))
+  {
+    MarshalledJournalRefinement.InvInit(v'.ephemeral.v, v.persistent);
+    MarshalledJournalRefinement.RefinementInit(v'.ephemeral.v, v.persistent);
+  }
+
+  lemma ReadForRecoveryRefines(v: Variables, v': Variables, lbl: TransitionLabel)
+    requires Inv(v) && Next(v, v', lbl) && lbl.ReadForRecoveryLabel?
+    ensures Inv(v') && CrashTolerantJournal.Next(I(v), I(v'), IALabel(lbl))
+  {
+    JournalChainedNext(v.ephemeral.v, v'.ephemeral.v, MarshalledJournal.ReadForRecoveryLabel(lbl.records));
+  }
+
+  lemma JournalChainedNext(j: MarshalledJournal.Variables, j': MarshalledJournal.Variables, lbl: MarshalledJournal.TransitionLabel)
+    requires MarshalledJournalRefinement.Inv(j)
+    requires MarshalledJournal.Next(j, j', lbl)
+    ensures MarshalledJournalRefinement.Inv(j')
+    ensures AbstractJournal.Next(IMJ(j), IMJ(j'), IAMJLabel(lbl))
+  {
+    MarshalledJournalRefinement.RefinementNext(j, j', lbl);
+    // TODO(jonh): inconsistent theorem naming: RefinementNext vs NextRefines
+    LinkedJournalRefinement.NextRefines(
+      MarshalledJournalRefinement.I(j),
+      MarshalledJournalRefinement.I(j'),
+      lbl.I());
+    PagedJournalRefinement.NextRefines(
+      LinkedJournalRefinement.I(MarshalledJournalRefinement.I(j)),
+      LinkedJournalRefinement.I(MarshalledJournalRefinement.I(j')),
+      lbl.I().I());
+  }
+
+//  lemma QueryEndLsnRefines(v: Variables, v': Variables, lbl: TransitionLabel)
+//    requires Inv(v) && Next(v, v', lbl) && lbl.QueryEndLsnLabel?
+//    ensures Inv(v') && CrashTolerantJournal.Next(I(v), I(v'), IALabel(lbl))
+//  {
+//  }
+
+  lemma PutRefines(v: Variables, v': Variables, lbl: TransitionLabel)
+    requires Inv(v) && Next(v, v', lbl) && lbl.PutLabel?
+    ensures Inv(v') && CrashTolerantJournal.Next(I(v), I(v'), IALabel(lbl))
+  {
+    MarshalledJournalRefinement.RefinementNext(v.ephemeral.v, v'.ephemeral.v, MarshalledJournal.PutLabel(lbl.records));
+  }
+
+//  lemma QueryLsnPersistenceRefines(v: Variables, v': Variables, lbl: TransitionLabel)
+//    requires Inv(v) && Next(v, v', lbl) && lbl.QueryLsnPersistenceLabel?
+//    ensures Inv(v') && CrashTolerantJournal.Next(I(v), I(v'), IALabel(lbl))
+//  {
+//  }
+
+  lemma InternalRefines(v: Variables, v': Variables, lbl: TransitionLabel)
+    requires Inv(v) && Next(v, v', lbl) && lbl.InternalLabel?
+    ensures Inv(v') && CrashTolerantJournal.Next(I(v), I(v'), IALabel(lbl))
+  {
+    JournalChainedNext(v.ephemeral.v, v'.ephemeral.v, MarshalledJournal.InternalLabel());
+
+    var lbl := MarshalledJournal.InternalLabel();
+    MarshalledJournalRefinement.RefinementNext(v.ephemeral.v, v'.ephemeral.v, lbl);
+      
+    if v'.inFlight.Some? {
+      var inFlightL := v.inFlight.value.I();
+      var ephemeralL := MarshalledJournalRefinement.I(v.ephemeral.v).truncatedJournal;
+      var discardedL := ephemeralL.DiscardOld(inFlightL.SeqStart());
+      LinkedJournalRefinement.BuildTightBuildsSubDisks(discardedL.diskView, discardedL.freshestRec);  // to pass lstep.addr membership through InFlightSubDiskProperty BuildTight
+
+      LinkedJournalRefinement.InFlightSubDiskPreserved(
+        MarshalledJournalRefinement.I(v.ephemeral.v),
+        MarshalledJournalRefinement.I(v'.ephemeral.v),
+        v.inFlight.value.I());
+    }
+    MarshalledJournalRefinement.TypedModelUnique(); // Completes persistent.IsSubDisk(ephemeral) proof.
+  }
+
+  lemma CommitStartRefines(v: Variables, v': Variables, lbl: TransitionLabel)
+    requires Inv(v) && Next(v, v', lbl) && lbl.CommitStartLabel?
+    ensures Inv(v') && CrashTolerantJournal.Next(I(v), I(v'), IALabel(lbl))
+  {
+    var frozenJournal := v'.inFlight.value;
+    JournalChainedNext(v.ephemeral.v, v'.ephemeral.v,
+      MarshalledJournal.FreezeForCommitLabel(frozenJournal));
+
+    var mjlbl := MarshalledJournal.FreezeForCommitLabel(frozenJournal);
+    MarshalledJournalRefinement.RefinementNext(v.ephemeral.v, v'.ephemeral.v, mjlbl);  // hoist one layer to LinkedJournal. (JournalChainedNext hides this jump)
+    LinkedJournalRefinement.InFlightSubDiskCreated(
+      MarshalledJournalRefinement.I(v.ephemeral.v),
+      MarshalledJournalRefinement.I(v'.ephemeral.v),
+      mjlbl.I());
+  }
+
+  lemma CommitCompleteRefines(v: Variables, v': Variables, lbl: TransitionLabel)
+    requires Inv(v) && Next(v, v', lbl) && lbl.CommitCompleteLabel?
+    ensures Inv(v') && CrashTolerantJournal.Next(I(v), I(v'), IALabel(lbl))
+  {
+    JournalChainedNext(v.ephemeral.v, v'.ephemeral.v,
+      MarshalledJournal.DiscardOldLabel(v.inFlight.value.SeqStart(), lbl.requireEnd));
+    MarshalledJournalRefinement.TypedModelUnique(); // Completes persistent.IsSubDisk(ephemeral) proof.
+    v.inFlight.value.I().I().BuildReceipt().BoundaryLSN();  // MJ label seqStarT is AbstractJournal label SeqStart
+  }
+
+  lemma CrashRefines(v: Variables, v': Variables, lbl: TransitionLabel)
+    requires Inv(v) && Next(v, v', lbl) && lbl.CrashLabel?
+    ensures Inv(v') && CrashTolerantJournal.Next(I(v), I(v'), IALabel(lbl))
+  {
+  }
+
+
+  lemma NextRefines(v: Variables, v': Variables, lbl: TransitionLabel)
+    requires Next(v, v', lbl)
+    requires Inv(v)
+    ensures Inv(v')
+    ensures CrashTolerantJournal.Next(I(v), I(v'), IALabel(lbl))
+  {
+    match lbl {
+      case LoadEphemeralFromPersistentLabel() => { LoadEphemeralFromPersistentRefines(v, v', lbl); }
+      case ReadForRecoveryLabel(_) => { ReadForRecoveryRefines(v, v', lbl); }
+      case QueryEndLsnLabel(_) => { /*QueryEndLsnRefines(v, v', lbl);*/ }
+      case PutLabel(_) => { PutRefines(v, v', lbl); }
+      case InternalLabel() => { InternalRefines(v, v', lbl); }
+      case QueryLsnPersistenceLabel(_) => { /*QueryLsnPersistenceRefines(v, v', lbl);*/ }
+      case CommitStartLabel(_, _) => { CommitStartRefines(v, v', lbl); }
+      case CommitCompleteLabel(_) => { CommitCompleteRefines(v, v', lbl); }
+      case CrashLabel() => { CrashRefines(v, v', lbl); }
+    }
+  }
+}
