Splinter/BlockLayer/BlockCrashTolerantMap.i.dfy
@@ -1,0 +1,181 @@
+// Copyright 2018-2021 VMware, Inc., Microsoft Inc., Carnegie Mellon University, ETH Zurich, and University of Washington
+// SPDX-License-Identifier: BSD-2-Clause
+
+include "../CoordinationLayer/CrashTolerantMap.i.dfy"
+
+// TODO(jonh): This is a copy-paste of Splinter/CoordinationLayer/CrashTolerantMap. Functor-reuse?
+
+module BlockCrashTolerantMap {
+  import opened ValueMessage
+  import opened KeyType
+  import opened StampedMapMod
+  import opened MsgHistoryMod
+  import opened LSNMod
+  import opened Options
+  import AbstractMap
+  import CrashTolerantMap
+
+  type TransitionLabel = CrashTolerantMap.TransitionLabel
+
+  type StoreImage = StampedMap
+
+  datatype Ephemeral =
+    | Unknown
+    | Known(v: AbstractMap.Variables)
+
+  datatype Variables = Variables(
+    persistent: StoreImage,
+    ephemeral: Ephemeral,
+    inFlight: Option<StoreImage>
+  )
+  {
+    predicate WF() {
+      true
+    }
+  }
+
+  predicate LoadEphemeralFromPersistent(v: Variables, v': Variables, lbl: TransitionLabel)
+  {
+    && v.WF()
+    && lbl.LoadEphemeralFromPersistentLabel?
+    && v.ephemeral.Unknown?
+    && v'.ephemeral.Known?
+
+    && lbl.endLsn == v.persistent.seqEnd
+    && AbstractMap.Init(v'.ephemeral.v, v.persistent)
+    && v'.persistent == v.persistent // UNCHANGED
+    && v'.inFlight == v.inFlight // UNCHANGED
+  }
+
+  predicate PutRecords(v: Variables, v': Variables, lbl: TransitionLabel)
+  {
+    && v.WF()
+    && lbl.WF()
+    && lbl.PutRecordsLabel?
+    && v.ephemeral.Known?
+    && v'.ephemeral.Known?
+  
+    && AbstractMap.Next(v.ephemeral.v, v'.ephemeral.v, AbstractMap.PutLabel(lbl.records))
+    && v'.persistent == v.persistent // UNCHANGED
+    && v'.inFlight == v.inFlight // UNCHANGED
+  }
+
+  predicate Query(v: Variables, v': Variables, lbl: TransitionLabel)
+  {
+    && v.WF()
+    && lbl.WF()
+    && lbl.QueryLabel?
+    && v.ephemeral.Known?
+    && v'.ephemeral.Known?
+
+    && AbstractMap.Next(v.ephemeral.v, v'.ephemeral.v, AbstractMap.QueryLabel(lbl.endLsn, lbl.key, lbl.value))
+    && v' == v
+  }
+
+  predicate FreezeMapInternal(v: Variables, v': Variables, lbl: TransitionLabel, frozenMap: StampedMap)
+  {
+    && v.WF()
+    && lbl.WF()
+    && lbl.InternalLabel?
+    && v.ephemeral.Known?
+    && v'.ephemeral.Known?
+    // Can't re-freeze until last in flight state reaches CommitComplete, since
+    // an async superblock write may be in progress, and we need to maintain
+    // guarantees about its in-flight map state.
+    && v.inFlight.None?
+
+    && AbstractMap.FreezeAs(v.ephemeral.v, v'.ephemeral.v, AbstractMap.FreezeAsLabel(frozenMap))
+    && v'.inFlight == Some(frozenMap)
+    && v'.persistent == v.persistent // UNCHANGED
+  }
+  
+  predicate EphemeralInternal(v: Variables, v': Variables, lbl: TransitionLabel)
+  {
+    && v.WF()
+    && lbl.WF()
+    && lbl.InternalLabel?
+    && v.ephemeral.Known?
+    && v'.ephemeral.Known?
+
+    && AbstractMap.Next(v.ephemeral.v, v'.ephemeral.v, AbstractMap.InternalLabel())
+    && v'.persistent == v.persistent // UNCHANGED
+    && v'.inFlight == v.inFlight // UNCHANGED
+  }
+
+  predicate CommitStart(v: Variables, v': Variables, lbl: TransitionLabel)
+  {
+    && v.WF()
+    && lbl.WF()
+    && lbl.CommitStartLabel?
+    && v.ephemeral.Known?
+    && v.inFlight.Some?
+
+    // Frozen map can't go backwards vs persistent map, lest we end up with
+    // a gap to the ephemeral journal start.
+    && v.persistent.seqEnd <= lbl.newBoundaryLsn
+    // Frozen journal & frozen map agree on boundary.
+    && lbl.newBoundaryLsn == v.inFlight.value.seqEnd
+
+    && v' == v
+  }
+
+  predicate CommitComplete(v: Variables, v': Variables, lbl: TransitionLabel)
+  {
+    && v.WF()
+    && lbl.WF()
+    && lbl.CommitCompleteLabel?
+    && v.inFlight.Some?
+
+    && v' == v.(
+      persistent := v.inFlight.value,
+      // ephemeral unchanged
+      inFlight := None)
+  }
+
+  predicate Crash(v: Variables, v': Variables, lbl: TransitionLabel)
+  {
+    && v.WF()
+    && lbl.WF()
+    && lbl.CrashLabel?
+    && v' == v.(
+      ephemeral := Unknown,
+      inFlight := None)
+  }
+
+  datatype Step =
+    | LoadEphemeralFromPersistentStep()
+    | PutRecordsStep()
+    | QueryStep()
+    | FreezeMapInternalStep(frozenMap: StampedMap)
+    | EphemeralInternalStep()
+    | CommitStartStep()
+    | CommitCompleteStep()
+    | CrashStep()
+
+
+  // Models mkfs
+  predicate Init(v: Variables)
+  {
+    v == Variables(StampedMapMod.Empty(), Unknown, None)
+  }
+
+  predicate NextStep(v: Variables, v': Variables, lbl: TransitionLabel, step: Step)
+  {
+    match step {
+      case LoadEphemeralFromPersistentStep() => LoadEphemeralFromPersistent(v, v', lbl)
+      case PutRecordsStep() => PutRecords(v, v', lbl)
+      case QueryStep() => Query(v, v', lbl)
+      case FreezeMapInternalStep(frozenMap) => FreezeMapInternal(v, v', lbl, frozenMap)
+      case EphemeralInternalStep() => EphemeralInternal(v, v', lbl)
+      case CommitStartStep() => CommitStart(v, v', lbl)
+      case CommitCompleteStep() => CommitComplete(v, v', lbl)
+      case CrashStep() => Crash(v, v', lbl)
+    }
+  }
+
+  predicate Next(v: Variables, v': Variables, lbl: TransitionLabel)
+  {
+    exists step :: NextStep(v, v', lbl, step)
+  }
+}
+
