Splinter/BlockLayer/BlockCrashTolerantMapRefinement.i.dfy
@@ -1,0 +1,80 @@
+// Copyright 2018-2021 VMware, Inc., Microsoft Inc., Carnegie Mellon University, ETH Zurich, and University of Washington
+// SPDX-License-Identifier: BSD-2-Clause
+
+include "BlockCrashTolerantMap.i.dfy"
+include "../CoordinationLayer/CrashTolerantMap.i.dfy"
+
+module BlockCrashTolerantMapRefinement {
+  import opened Options
+  import opened ValueMessage
+  import opened KeyType
+  import opened StampedMapMod
+  import opened MsgHistoryMod
+  import opened LSNMod
+  import CrashTolerantMap 
+  import opened BlockCrashTolerantMap 
+
+  predicate DecodableImage(store: StoreImage)
+  {
+    true
+  }
+
+  function IImage(store: StoreImage) : CrashTolerantMap.StoreImage
+    requires DecodableImage(store)
+  {
+    store
+  }
+
+  predicate Decodable(v: Variables)
+  {
+    true
+  }
+
+  function I(v: Variables) : CrashTolerantMap.Variables
+    requires Decodable(v)
+  {
+    CrashTolerantMap.Variables(
+      IImage(v.persistent),
+      if v.ephemeral.Unknown?
+      then CrashTolerantMap.Unknown
+      else CrashTolerantMap.Known(
+        v.ephemeral.v
+      ),
+      if v.inFlight.None? then None else Some(IImage(v.inFlight.value))
+    )
+  }
+
+  predicate Inv(v: Variables)
+  {
+    && Decodable(v)
+  }
+
+  function IALabel(lbl: TransitionLabel) : CrashTolerantMap.TransitionLabel
+    requires lbl.WF()
+  {
+    lbl
+  }
+
+  function IStep(step: Step) : CrashTolerantMap.Step
+  {
+    match step
+      case LoadEphemeralFromPersistentStep() => CrashTolerantMap.LoadEphemeralFromPersistentStep()
+      case PutRecordsStep() => CrashTolerantMap.PutRecordsStep()
+      case QueryStep() => CrashTolerantMap.QueryStep()
+      case FreezeMapInternalStep(frozenMap) => CrashTolerantMap.FreezeMapInternalStep(frozenMap)
+      case EphemeralInternalStep() => CrashTolerantMap.EphemeralInternalStep()
+      case CommitStartStep() => CrashTolerantMap.CommitStartStep()
+      case CommitCompleteStep() => CrashTolerantMap.CommitCompleteStep()
+      case CrashStep() => CrashTolerantMap.CrashStep()
+  }
+
+  lemma NextRefines(v: Variables, v': Variables, lbl: TransitionLabel)
+    requires Next(v, v', lbl)
+    requires Inv(v)
+    ensures Inv(v')
+    ensures CrashTolerantMap.Next(I(v), I(v'), IALabel(lbl))
+  {
+    var step :| NextStep(v, v', lbl, step);
+    assert CrashTolerantMap.NextStep(I(v), I(v'), IALabel(lbl), IStep(step));
+  }
+}
